try to use program fixpoint and stronly induction to prove decode_instrs

elf/SymbtableDecode.v
@@ -1,8 +1,9 @@
-Require Import Coqlib Integers AST Maps.
+Require Import Coqlib Integers String AST Maps.
 Require Import Asm Errors.
 Require Import RelocProg RelocProgram Encode.
 Require Import Memdata.
-Require Import encode.Hex encode.Bits.
+Require Import Hex encode.Bits.
+Import Hex Bits.
 Import ListNotations.
 Require Import SymbtableEncode.
 
@@ -10,7 +11,7 @@ Set Implicit Arguments.
 
 Local Open Scope error_monad_scope.
 Local Open Scope hex_scope.
-Local Open Scope bits_scope.
+Local Open Scope string_scope.
 
 Definition decode_symbtype (z: Z) : res symbtype :=
   match z with
@@ -39,3 +40,113 @@ Lemma decode_encode_bindtype bt:
 Proof.
   destruct bt; reflexivity.
 Qed.
+
+
+Definition decode_glob_symb_info (z: Z) :=
+  let st := z mod 16 in
+  let bt := z / 16 in
+  do st <- decode_symbtype st;
+    do bt <- decode_bindtype bt;
+    OK (st, bt).
+
+Lemma decode_encode_glob_symb_info st bt :
+  decode_glob_symb_info (encode_glob_symb_info bt st) = OK (st, bt).
+Proof.
+  unfold decode_glob_symb_info, encode_glob_symb_info.
+  change (2 ^ 4) with 16.
+  rewrite Z.add_comm, Z_mod_plus_full, <- Z.add_comm.
+  rewrite Z_div_plus_full_l by lia.
+  rewrite Z.div_small, Z.mod_small, Z.add_0_r.
+  rewrite decode_encode_symbtype, decode_encode_bindtype. reflexivity.
+  destruct st; simpl; lia.
+  destruct st; simpl; lia.
+Qed.
+
+
+
+Definition decode_secindex (lb: list byte) (m: ZTree.t ident) : res secindex :=
+  let i := decode_int lb in
+  if zeq i HZ["FFF2"]
+  then OK secindex_comm
+  else if zeq i 0
+       then OK secindex_undef
+       else
+         match ZTree.get i m with
+         | Some id =>
+           OK (secindex_normal id)
+         | _ => Error (msg "no ident in map to secindex")
+         end.
+
+Definition match_idxmap (m1:PTree.t Z) (m2: ZTree.t ident) :=
+  forall id z (H: m1 ! id = Some z), ZTree.get z m2 = Some id.
+
+Lemma decode_encode_secindex: forall i bs m1 m2 (M: match_idxmap m1 m2),    
+    encode_secindex i m1 = OK bs ->
+    decode_secindex bs m2 = OK i.
+Proof.
+  unfold decode_secindex, encode_secindex, match_idxmap.
+  intros.
+  destr_in H.
+  - destr_in H. destr_in H.
+    apply andb_true_iff in Heqb. simpl in Heqb.
+    destruct Heqb as (A & B).
+    apply Z.ltb_lt in A.  apply Z.ltb_lt in B.
+    simpl. inv H. rewrite decode_encode_int.        
+    simpl. rewrite Z.mod_small.
+    rewrite pred_dec_false. rewrite pred_dec_false.
+    erewrite M;eauto. lia. lia. change (two_power_pos 16) with 65536.
+    lia.
+  - inv H. rewrite decode_encode_int.
+    simpl. auto.
+  - inv H. rewrite decode_encode_int. 
+    simpl. auto.
+Qed.
+
+Definition decode_symbentry32 (lb: list byte) (m: ZTree.t ident): res symbentry :=
+  do (st_name_bytes, lb) <- take_drop 4 lb;
+  do (st_value_bytes, lb) <- take_drop 4 lb;
+  do (st_size_bytes, lb) <- take_drop 4 lb;
+  do (st_info_bytes, lb) <- take_drop 1 lb;
+  do (st_other_bytes, lb) <- take_drop 1 lb;
+  do (st_shndx_bytes, lb) <- take_drop 2 lb;
+
+  let svalue := decode_int32 st_value_bytes in
+  let ssize := decode_int32 st_size_bytes in
+  do (st, bt) <- decode_glob_symb_info (decode_int st_info_bytes);
+  do secindex <- decode_secindex st_shndx_bytes m;
+  OK (
+      {|
+        symbentry_bind := bt;
+        symbentry_type := st;
+        symbentry_value := svalue;
+        symbentry_secindex := secindex;
+        symbentry_size := ssize
+      |}
+    ).
+
+Definition decode_symbentry64 (lb: list byte) (m: ZTree.t ident): res symbentry :=
+  do (st_name_bytes, lb) <- take_drop 4 lb;
+  do (st_value_bytes, lb) <- take_drop 8 lb;
+  do (st_size_bytes, lb) <- take_drop 8 lb;
+  do (st_info_bytes, lb) <- take_drop 1 lb;
+  do (st_other_bytes, lb) <- take_drop 1 lb;
+  do (st_shndx_bytes, lb) <- take_drop 2 lb;
+
+  let svalue := decode_int st_value_bytes in
+  let ssize := decode_int st_size_bytes in
+  do (st, bt) <- decode_glob_symb_info (decode_int st_info_bytes);
+  do secindex <- decode_secindex st_shndx_bytes m;
+  OK (
+      {|
+        symbentry_bind := bt;
+        symbentry_type := st;
+        symbentry_value := svalue;
+        symbentry_secindex := secindex;
+        symbentry_size := ssize
+      |}
+    ).
+
+Lemma decode_encode_symbentry32 : forall e bs nidx m1 m2 (M: match_idxmap m1 m2),
+    encode_symbentry32 e nidx m1 = OK bs ->
+    decode_symbentry32 bs m2 = OK e.
+Admitted.
